#+hugo_base_dir: /home/phihungnguyen/blog/secondbrain
* Deutsch's Problem
:PROPERTIES:
:EXPORT_FILE_NAME: deutsch_problem
:ID:       9aef3386-da89-40f4-baae-76c05b109a3c
:END:
#+title: deutsch



Look at [[id:37409b01-071d-4cca-b3bb-7ba1b46845e8la][Query Gate]] 
#+BEGIN_SRC latex
\documentclass{article}
\begin{document}
Hello, LaTeX!
$n \in x$
\end{document}
#+END_SRC


#+BEGIN_LaTeX
\section{Introduction}
This is LaTeX content directly within Org mode. You can write your LaTeX code here.

\begin{equation}
E = mc^2
\end{equation}
#+END_LaTeX

Learn about the query here:
Deustch's algorithm solves the parity problem for \(n=1\).

Deutsch's problem:

Input: a function \( f:\{0,1\} \to \{0,1\} \)

Output: 0 if f is constant, 1 if f is balanced

The quantum circuit looks like this :

...

The initial state is \(\ket{0}\ket{1}\), by applying two hadamard gates:

\begin{align*}
	H \otimes H \ket{1} \ket{0} &= \ket{-} \ket{+} \\
&= \frac{1}{\sqrt{2}}(\ket{0} + \ket{1}) \frac{1}{2}(\ket{0} - \ket{1}) \\
&= \frac{1}{2}(\ket{0} - \ket{1}) \ket{0} + \frac{1}{2}(\ket{0} - \ket{1})\ket{1}
&= \ket{\psi_1}
\end{align*}

$ \ket{\psi_1} \ket{\psi_2}$

Next, we apply the $U_f$ gate:
and we can as well utilize this expression
$ \ket{0 \otimes a} - \ket{1 \otimes a} = (-1)^a (\ket{0} - \ket{1})$ 

\begin{align*}
	U_f  \ket{\psi_1}
&= \frac{1}{2}(\ket{0 \otimes f(0)} - \ket{1 \otimes f(0)})\ket{0}
+ \frac{1}{2}(\ket{0 \otimes f(0) - \ket{1 \otimes f(1)}})\ket{1} \\
&= \frac{1}{2}(-1)^{f(0)}(\ket{0} - \ket{1})\ket{0}
+ \frac{1}{2}(-1)^{f(1)}(\ket{0} - \ket{1})\ket{1} \\
&= \ket{-} \left( \frac{(-1)^{f(0)} \ket{0} + (-1)^{f(1)} \ket{1}}{\sqrt{2}} \right)
\end{align*}


A phase kickback happened here: learn more at


So finally, we obtained

\begin{align*}
	\ket{\psi_2} &= (-1)^{f(0)}\ket{-} \left( \frac{\ket{0} + (-1)^{f(0) \otimes f(1)}\ket{1}}{\sqrt{2}} \right) \\
&=
   \begin{cases}
        (-1)^{f(0)} \ket{-} \ket{+} \quad \text{if} f(0) \otimes f(1) = 0\\
        (-1)^{f(0)} \ket{-} \ket{-} \quad \text{if} f(0) \otimes f(1) = 1
   \end{cases}
\end{align*}


After applying the hadamard again, we obtain the final solution:

\begin{align*}
	\ket{\psi_3} &=
\begin{cases}
   (-1)^{f(0)} \ket{-} \ket{0} \quad \text{if} f(0) \otimes f(1) = 0\\
   (-1)^{f(0)} \ket{-} \ket{1} \quad \text{if} f(0) \otimes f(1) = 1
\end{cases}
\end{align*}

